adding well-typed ext blocks bir_typing_prog; removes further `mem_core_*`

src/theory/tools/promising/bir_mem_coreSyntax.sig
@@ -1,8 +1,0 @@
-signature bir_mem_coreSyntax =
-sig
-   include Abbrev
-
-
-   val mem_init_tm      : term;
-
-end
